investigations/bedrock2/Aes/Aes.v
@@ -33,7 +33,8 @@ Section Impl.
     let aes_cfg_manual_operation := "aes_cfg_manual_operation" in
     let cfg_val := "cfg_val" in
     ("b2_aes_init",
-     (globals ++ [aes_cfg_operation; aes_cfg_mode; aes_cfg_key_len],
+     (globals ++ [aes_cfg_operation; aes_cfg_mode; aes_cfg_key_len;
+                 aes_cfg_manual_operation],
       [], bedrock_func_body:(
       output! WRITE (AES_CTRL,
                      ((aes_cfg_operation << AES_CTRL_OPERATION) |
