investigations/bedrock2/Aes/AesProperties.v
@@ -1,0 +1,283 @@
+Require Import Coq.Strings.String.
+Require Import Coq.Lists.List.
+Require Import Coq.micromega.Lia.
+Require Import Coq.ZArith.ZArith.
+Require Import bedrock2.ProgramLogic.
+Require Import bedrock2.Semantics.
+Require Import bedrock2.Syntax.
+Require Import bedrock2.TailRecursion.
+Require Import bedrock2.WeakestPrecondition.
+Require Import bedrock2.WeakestPreconditionProperties.
+Require Import coqutil.Word.Interface.
+Require Import coqutil.Word.Properties.
+Require Import coqutil.Map.Interface.
+Require Import coqutil.Tactics.Tactics.
+Require Import coqutil.Tactics.letexists.
+Require Import Bedrock2Experiments.Aes.AesSemantics.
+Require Import Bedrock2Experiments.Aes.Aes.
+Import Syntax.Coercions List.ListNotations.
+Local Open Scope Z_scope.
+
+Section Proofs.
+  Context {p : parameters} {p_ok : parameters.ok p}
+          {consts : constants word.rep} {consts_ok : constants.ok consts}
+          {timing : timing}.
+  Import constants parameters.
+
+  (***** General-purpose lemmas/tactics and setup *****)
+
+  Add Ring wring : (Properties.word.ring_theory (word := Semantics.word))
+        (preprocess [autorewrite with rew_word_morphism],
+         morphism (Properties.word.ring_morph (word := Semantics.word)),
+         constants [Properties.word_cst]).
+
+  Existing Instance constants.constant_names | 10.
+
+  Lemma interact_mmio call action binds arges t m l (post : trace -> mem -> locals -> Prop) args :
+    dexprs m l arges args ->
+    (forall s s' rets,
+        execution t s ->
+        step action s args rets s' ->
+        (exists l0 : locals,
+            map.putmany_of_list_zip binds rets l = Some l0 /\
+            post ((map.empty, action, args, (map.empty, rets)) :: t) m l0)) ->
+    cmd call (cmd.interact binds action arges) t m l post.
+  Proof.
+    intros. eapply interact_nomem; [ eassumption | ].
+    cbn [Semantics.ext_spec semantics_parameters].
+    cbv [ext_spec]. split; [reflexivity | ].
+    intros. split; [ reflexivity | ].
+    cbn [execution] in *; destruct_products.
+    eauto.
+  Qed.
+
+  Local Ltac subst1_map m :=
+    match m with
+    | map.put ?m _ _ => subst1_map m
+    | ?m => is_var m; subst m
+    end.
+
+  Local Ltac map_lookup :=
+    repeat lazymatch goal with
+           | |- context [map.get ?l] =>
+             try apply map.get_put_same; try eassumption;
+             subst1_map l;
+             rewrite ?map.get_put_diff by congruence
+           end.
+
+  Local Ltac straightline_with_map_lookup :=
+    lazymatch goal with
+    | |- exists v, map.get _ _ = Some v /\ _ =>
+      eexists; split; [ solve [map_lookup] | ]
+    | _ => straightline
+    end.
+
+  Local Ltac interaction :=
+    eapply interact_mmio; [ solve [repeat straightline_with_map_lookup] | ];
+    repeat straightline;
+    lazymatch goal with
+    | H : step _ _ _ _ _ |- _ => inversion H; clear H; subst
+    end.
+
+  Hint Extern 4 (step _ ?s _ _ _) => eapply (ReadStep s) : step.
+  Hint Extern 4 (step _ ?s _ _ _) => eapply (WriteStep s) : step.
+  Hint Constructors read_step : step.
+  Hint Constructors write_step : step.
+
+  Local Ltac simplify_unique_words_in H :=
+    lazymatch type of H with
+    | unique_words ?words =>
+      let H' := fresh in
+      cbv [unique_words] in H;
+      pose proof (List.NoDup_dedup word.eqb words) as H';
+      rewrite H in H'; clear H;
+      repeat lazymatch goal with
+             | H : List.NoDup [] |- _ => clear H
+             | H : List.NoDup (_ :: _) |- _ => inversion H; clear H; subst; cbv [List.In] in *
+             | H : ~ (_ \/ _) |- _ => apply Decidable.not_or in H
+             | H : _ /\ _ |- _ => destruct H
+             end
+    | ?t => fail "expected hypothesis of type [unique_words _], got one of type" t
+    end.
+
+  Local Ltac one_goal_or_solved t :=
+    solve [t] || (t; [ ]).
+
+  Local Ltac invert_nobranch' H t :=
+    first [ inversion H; clear H; subst; solve [t]
+          | inversion H; clear H; subst; t; [ ] ].
+  Local Ltac invert_nobranch H :=
+    invert_nobranch' H ltac:(try congruence).
+
+  (* TODO: implement register naming with separation logic? e.g.
+
+     (Register addr val * Register addr2 val2 * ...) regs
+
+     Then inductive rules could say (Register addr val * R) regs
+   *)
+  Lemma reg_addr_unique r1 r2 : reg_addr r1 = reg_addr r2 -> r1 = r2.
+  Proof.
+    assert (forall w, word.add w (word.of_Z 0) = w) as word_add_0
+        by (intros; ring).
+    pose proof addrs_unique (ok:=consts_ok) as Huniq.
+    cbv [all_reg_addrs list_reg_addrs] in *.
+    rewrite nregs_key_eq, nregs_iv_eq, nregs_data_eq in Huniq.
+    repeat lazymatch type of Huniq with
+           | context [Z.to_nat ?n] =>
+             let x := constr:(Z.to_nat n) in
+             let y := (eval vm_compute in x) in
+             change x with y in Huniq
+           end.
+    cbn in Huniq. simplify_unique_words_in Huniq.
+    rewrite !word_add_0 in *. clear word_add_0.
+    cbv [reg_addr]; intro Heqaddr.
+    destruct r1.
+    (* clear all hypothesis that don't have to do with r1 (makes proof
+       faster) *)
+    all:lazymatch type of Heqaddr with
+        | ?r = _ =>
+          repeat match goal with
+                 | H : ?x <> ?y |- _ =>
+                   lazymatch x with
+                   | context [r] => fail
+                   | _ =>
+                     lazymatch y with
+                     | context [r] => fail
+                     | _ => clear H
+                     end
+                   end
+                 end
+        end.
+    all:destruct r2; first [ exact eq_refl | congruence ].
+  Qed.
+
+  Local Ltac invert_bool :=
+    lazymatch goal with
+    | H : (_ && _)%bool = true |- _ =>
+      apply Bool.andb_true_iff in H; destruct H
+    | H : (_ && _)%bool = false |- _ =>
+      apply Bool.andb_false_iff in H; destruct H
+    | H : negb _ = true |- _ =>
+      apply Bool.negb_true_iff in H
+    | H : negb _ = false |- _ =>
+      apply Bool.negb_false_iff in H
+    end.
+
+  Lemma execution_unique (t : trace) s1 s2 :
+    execution t s1 ->
+    execution t s2 ->
+    s1 = s2.
+  Proof.
+    pose proof status_flags_unique_and_nonzero (ok:=consts_ok) as Hflags.
+    cbv [map] in Hflags.
+    simplify_unique_words_in Hflags.
+    revert s1 s2.
+    induction t; cbn [execution]; [ congruence | ].
+    intros; destruct_products.
+    match goal with
+    | H1 : execution t ?s1, H2 : execution t ?s2 |- _ =>
+      specialize (IHt _ _ H1 H2); subst
+    end.
+    repeat (lazymatch goal with
+            | x := _ |- _ => subst x
+            | |- ?x = ?x => reflexivity
+            | H : is_busy (BUSY _ _ _) = false |- _ =>
+              cbv [is_busy] in H; exfalso; congruence
+            | H : reg_addr _ = reg_addr _ |- _ =>
+              apply reg_addr_unique in H; subst
+            | H : step _ _ _ _ _ |- _ =>
+              inversion H; clear H; subst
+            | H : read_step _ _ _ _ |- _ =>
+              inversion H; clear H; subst
+            | H : write_step _ _ _ _ |- _ =>
+              inversion H; clear H; subst
+            | _ => first [ invert_bool
+                        | progress cbn [status_matches_state is_output_reg] in *]
+            end; try congruence).
+  Qed.
+
+  Lemma word_wrap_unsigned w : word.wrap (word.unsigned w) = word.unsigned w.
+  Proof.
+    pose proof (word.unsigned_range w).
+    cbv [word.wrap]. apply Z.mod_small; lia.
+  Qed.
+
+  Local Ltac infer :=
+    repeat match goal with
+           | H : reg_addr _ _ |- _ => invert_nobranch H
+           | H : read_step _ _ _ _ |- _ => invert_nobranch H
+           | H : write_step _ _ _ _ |- _ => invert_nobranch H
+           | H : execution _ (DONE _) |- _ => invert_nobranch H; destruct_products
+           | H : step _ _ _ _ (DONE _) |- _ => invert_nobranch H
+           | H1 : execution ?t _, H2 : execution ?t _ |- _ =>
+             pose proof execution_unique _ _ _ H1 H2; subst;
+             clear H2; one_goal_or_solved ltac:(try congruence)
+           | H : BUSY _ _ = BUSY _ _ |- _ => invert_nobranch H
+           | H : ?x = ?x |- _ => clear H
+           end.
+
+  Hint Rewrite word.unsigned_add word.unsigned_sub word.unsigned_mul
+       word.unsigned_mulhuu word.unsigned_divu word.unsigned_and
+       word.unsigned_or word.unsigned_xor word.unsigned_sru word.unsigned_slu
+       word.unsigned_ltu @word.unsigned_of_Z_0 @word.unsigned_of_Z_1
+       using solve [typeclasses eauto] : push_unsigned.
+
+  Lemma execution_step action args rets t s s':
+    execution t s -> step action s args rets s' ->
+    execution ((map.empty, action, args, (map.empty, rets)) :: t) s'.
+  Proof. intros; cbn [execution]; eauto. Qed.
+
+  (***** Proofs for specific functions *****)
+
+  (* plug in implicits (otherwise [straightline] fails) *)
+  Definition aes_init := aes_init.
+
+  Definition ctrl_value
+             (cfg_operation cfg_mode cfg_key_len cfg_manual_operation : word) :=
+    word.or
+      (word.or
+         (word.or (word.slu cfg_operation AES_CTRL_OPERATION)
+                  (word.slu (word.and cfg_mode AES_CTRL_MODE_MASK) AES_CTRL_MODE_OFFSET))
+         (word.slu (word.and cfg_key_len AES_CTRL_KEY_LEN_MASK) AES_CTRL_KEY_LEN_OFFSET))
+      (word.slu cfg_manual_operation AES_CTRL_MANUAL_OPERATION).
+
+  Instance spec_of_aes_init : spec_of aes_init :=
+    fun function_env =>
+      forall (tr : trace) (m : mem) (R : _ -> Prop)
+        aes_cfg_operation aes_cfg_mode aes_cfg_key_len
+        aes_cfg_manual_operation,
+        (* no special requirements of the memory *)
+        R m ->
+        (* circuit must start in UNINITIALIZED state *)
+        execution tr UNINITIALIZED ->
+        let args := [aes_cfg_operation; aes_cfg_mode; aes_cfg_key_len;
+                    aes_cfg_manual_operation] in
+        call function_env aes_init tr m (globals ++ args)
+             (fun tr' m' rets =>
+                (* the circuit is in IDLE state with the correct control
+                   register value and no other known register values *)
+                execution tr'
+                          (IDLE (map.put
+                                   map.empty AES_CTRL
+                                   (ctrl_value aes_cfg_operation aes_cfg_mode
+                                               aes_cfg_key_len
+                                               aes_cfg_manual_operation)))
+                (* ...and the same properties as before hold on the memory *)
+                /\ R m'
+                (* ...and there is no output *)
+                /\ rets = []).
+
+  Lemma aes_init_correct :
+    program_logic_goal_for_function! aes_init.
+  Proof.
+    (* initial processing *)
+    repeat straightline.
+
+    (* write CTRL *)
+    interaction; repeat straightline.
+
+    (* done; prove postcondition *)
+    ssplit; auto; [ ].
+    infer. eapply execution_step; eauto with step.
+  Qed.
+End Proofs.
